Bdd/Choice.lean
@@ -1,0 +1,121 @@
+import Bdd.Basic
+
+namespace Choice
+
+open Pointer
+open OBdd
+
+def choice_helper (O : OBdd n m) : O.1.root = .node j → Vector Bool n → Vector Bool n := fun hj I ↦
+  match hl : O.1.heap[j].low with
+  | .node j => choice_helper (O.low hj) hl I
+  | .terminal true => I.set O.1.heap[j].var false
+  | .terminal false =>
+    match hh : O.1.heap[j].high with
+    | .terminal _ => I.set O.1.heap[j].var true
+    | .node j' => (choice_helper (O.high hj) hh I).set O.1.heap[j].var true
+termination_by O
+
+def choice (O : OBdd n m) : (∃ I, O.evaluate I) → Vector Bool n := fun ht ↦
+  match O_root_def : O.1.root with
+  | .terminal true => Vector.replicate n false
+  | .terminal false => by
+    absurd ht
+    rw [OBdd.evaluate_terminal' O_root_def]
+    simp only [Function.const_apply, Bool.false_eq_true, exists_const, not_false_eq_true]
+  | .node j => choice_helper O O_root_def (Vector.replicate n false)
+
+private lemma Vector.get_set_ne {xs : Vector α n} {x : α} (hi : i < n) {j : Fin n} (h : i ≠ j) :
+    (xs.set i x hi).get j = xs.get j := by
+  simp only [Vector.get]
+  aesop
+
+def choice_helper_spec' {O : OBdd n m} (hr : O.Reduced) (hj : O.1.root = .node j) (i : Fin n) :
+    i < O.1.heap[j].var → (choice_helper O hj (Vector.replicate n false)).get i = false := by
+  intro hi
+  unfold choice_helper
+  split
+  next jl hl =>
+    have := var_lt_low_var (h := hj)
+    simp only [var, Nat.succ_eq_add_one, Bdd.var, hj, toVar_node_eq, Fin.coe_eq_castSucc, Fin.coe_castSucc, low, Bdd.low, hl, toVar] at this
+    apply choice_helper_spec' (low_reduced hr)
+    simp_all
+    omega
+  next hl => simp [Vector.get]
+  next hl =>
+    split
+    next bh hh =>
+      simp [Vector.get]
+      rw [Array.getElem_set_ne]
+      · simp
+      · simp
+      · apply ne_of_gt
+        exact hi
+    next jh hh =>
+      have := var_lt_high_var (h := hj)
+      simp only [var, Nat.succ_eq_add_one, Bdd.var, hj, toVar_node_eq, Fin.coe_eq_castSucc, Fin.coe_castSucc, high, Bdd.high, hh, toVar] at this
+      rw [Vector.get_set_ne]
+      apply choice_helper_spec' (high_reduced hr)
+      · simp_all
+        omega
+      · omega
+termination_by O
+
+def choice_helper_spec'' {O : OBdd n m} (hr : O.Reduced) (hj : O.1.root = node j) (i : Fin n) :
+    i < O.1.heap[j].var → (choice_helper O hj (Vector.replicate n false))[i] = false := by
+  have := choice_helper_spec' hr hj i
+  exact this
+
+def choice_helper_spec {O : OBdd n m} (hr : O.Reduced) (hj : O.1.root = node j) :
+    O.evaluate (choice_helper O hj (Vector.replicate n false)) := by
+  unfold choice_helper
+  split
+  next jl hl =>
+    rw [evaluate_node'' hj]
+    simp only
+    suffices s : (choice_helper (O.low hj) hl (Vector.replicate n false))[O.1.heap[j].var] = false by
+      rw [s]
+      simp only [Bool.false_eq_true, ↓reduceIte]
+      apply choice_helper_spec (low_reduced hr)
+    rw [choice_helper_spec'' (low_reduced hr) hl]
+    have := var_lt_low_var (h := hj)
+    simp only [var, Nat.succ_eq_add_one, Bdd.var, toVar, hj, hl, Fin.coe_eq_castSucc, Fin.coe_castSucc, low, Bdd.low] at this
+    simp_all
+  next hl =>
+    rw [evaluate_node'' hj]
+    have : (O.low hj).1.root = terminal true := by simp only [low, Bdd.low, hl]
+    simp [evaluate_terminal' this]
+  next hl =>
+    split
+    next bh hh =>
+      rw [evaluate_node'' hj]
+      have : (O.high hj).1.root = terminal true := by
+        simp only [high, Bdd.high]
+        rw [hh]
+        congr
+        cases bh with
+        | false => exact False.elim (hr.1 ⟨node j, by simp_all; left⟩ ⟨by simp_all⟩)
+        | true => rfl
+      simp [evaluate_terminal' this]
+    next jh hh =>
+      rw [evaluate_node'' hj]
+      simp only [Fin.getElem_fin, Vector.getElem_set_self, ↓reduceIte]
+      have : (O.high hj).evaluate ((choice_helper (O.high hj) hh (Vector.replicate n false)).set O.1.heap[j.1].var.1 true) =
+             (O.high hj).evaluate (choice_helper (O.high hj) hh ((Vector.replicate n false))) := by
+        rw [Independence' (O.high hj) ⟨O.1.heap[j.1].var.1, ?_⟩ true (choice_helper (O.high hj) hh (Vector.replicate n false))]
+        rw [show O.1.heap[j.1].var.1 = O.var by simp [hj]]
+        exact var_lt_high_var
+      rw [this]
+      apply choice_helper_spec (high_reduced hr)
+termination_by O
+
+def choice_spec {O : OBdd n m} (hr : O.Reduced) (ht : ∃ I, O.evaluate I) : O.evaluate (choice O ht) := by
+  simp only [choice]
+  split
+  next O_root_def => rw [evaluate_terminal' O_root_def]; simp
+  next O_root_def =>
+    absurd ht
+    rw [evaluate_terminal' O_root_def]
+    simp only [Function.const_apply, Bool.false_eq_true, exists_const, not_false_eq_true]
+  next j O_root_def => exact choice_helper_spec hr O_root_def
+
+end Choice
